Syntax: share basic sort combinators
Much of our binding theory can be defined once for both languages in terms of
these definitions.

theories/prelude.v
@@ -3,8 +3,80 @@ From iris.algebra Require Export base.
 From Autosubst Require Export Autosubst.
 
 Definition stamp := positive.
+(* Not an instance because it should *not* be used automatically. *)
 Definition inh_ids `{Inhabited X}: Ids X := λ _, inhabitant.
-Instance ids_list {A}: Ids (list A) := inh_ids.
+Instance list_ids {X}: Ids (list X) := inh_ids.
+
+Section rename_instances.
+  Context `{Ids X} `{Rename X}.
+  Global Instance list_rename: Rename (list X) :=
+    λ sb, map (rename sb).
+  Definition list_rename_fold (sb : var → var) (xs : list X) : map (rename sb) xs = rename sb xs := eq_refl.
+  (* Hint Rewrite @list_rename_fold : autosubst. *)
+End rename_instances.
+
+Section subst_instances.
+  Context `{Ids vl} `{Subst vl} `{SubstLemmas vl}.
+  Context `{Ids X} `{Rename X} `{HSubst vl X} {hsl: HSubstLemmas vl X}.
+
+  Global Instance vls_hsubst: HSubst vl (list vl) :=
+    λ sb, map (subst sb).
+  Global Instance list_hsubst: HSubst vl (list X) :=
+    λ sb, map (hsubst sb).
+  Global Arguments list_hsubst /.
+  Global Arguments vls_hsubst /.
+
+  Definition vls_subst_fold (sb : var → vl) (vs : list vl) : map (subst sb) vs = hsubst sb vs := eq_refl.
+  Definition list_hsubst_fold sb (xs : list X) : map (hsubst sb) xs = hsubst sb xs := eq_refl.
+
+  Hint Rewrite @vls_subst_fold @list_hsubst_fold : autosubst.
+
+  Global Instance hsubst_lemmas_vls: HSubstLemmas vl (list vl).
+  Proof.
+    split; trivial; intros; rewrite /hsubst;
+      induction s; asimpl; by f_equal.
+  Qed.
+  Global Instance hsubst_lemmas_list: HSubstLemmas vl (list X).
+  Proof.
+    split; trivial; intros; rewrite /hsubst;
+      induction s; asimpl; by f_equal.
+  Qed.
+  Section pair_instances.
+    Context `{Inhabited A}.
+    Implicit Types (x: X) (a: A).
+
+    (** [Sort X → Sort (A, X)] *)
+    Definition mapsnd `(f: B → C) : A * B → A * C := λ '(a, b), (a, f b).
+    Global Instance pair_ids: Ids (A * X) := λ n, (inhabitant, ids n).
+    Global Instance pair_rename: Rename (A * X) :=
+      λ sb, mapsnd (rename sb).
+    Global Instance pair_hsubst: HSubst vl (A * X) :=
+      λ sb, mapsnd (hsubst sb).
+    Global Arguments pair_hsubst /.
+
+    Definition pair_rename_fold sb (ax: A * X): mapsnd (rename sb) ax = rename sb ax := eq_refl.
+    Definition pair_hsubst_fold sb (ax: A * X): mapsnd (hsubst sb) ax = hsubst sb ax := eq_refl.
+
+    Global Instance hsubst_lemmas_pair: HSubstLemmas vl (A * X).
+    Proof.
+      split; intros; rewrite /hsubst /pair_hsubst /mapsnd /=;
+        repeat case_match; simplify_eq; asimpl; by [].
+    Qed.
+    Definition list_pair_rename_fold sb (axs: list (A * X)): map (mapsnd (rename sb)) axs = rename sb axs := eq_refl.
+
+    Lemma list_pair_swap_snd_rename r axs: map snd (rename r axs) = map (rename r) (map snd axs).
+    Proof.
+      rewrite !map_map; elim: axs => [//| [a x] axs IHaxs /=]. by f_equal.
+    Qed.
+  End pair_instances.
+End subst_instances.
+Definition list_pair_hsubst_fold {A} `{HSubst vl X} sb (xs: list (A * X)): map (mapsnd (hsubst sb)) xs = hsubst sb xs := eq_refl.
+
+Global Hint Rewrite @vls_subst_fold @list_hsubst_fold : autosubst.
+(* The hints in the previous line are needed; for the next ones, that's less clear. *)
+Global Hint Rewrite @pair_rename_fold @pair_hsubst_fold : autosubst.
+Global Hint Rewrite @list_rename_fold @list_hsubst_fold : autosubst.
+Global Hint Rewrite @list_pair_rename_fold @list_pair_hsubst_fold : autosubst.
 
 (* Now type inference solves HSubst vl ? by infering HSubst vl ty infers unspecified asts to be [path]s. *)
 (* Goal ∀ s x, x.|[s] = x. *)
